doing some ravana stuff

ironfleet/ravana/Node.i.dfy
@@ -3,12 +3,81 @@ include "Types.i.dfy"
 module Protocol_Node_i {
   import opened Types_i
 
-  datatype Node = NodeController(
-                      leader: bool,
-                      controllerState: ControllerState,
-                | NodeSwitch(
-                      bufferedMessages: seq<S2C_Message>,
-                      switchState: SwitchState,
+  datatype Config = Config(
+      node_logger: EndPoint,
+      node_controllers: seq<EndPoint>,
+      node_switches: seq<EndPoint>
+    )
 
-   
+  datatype Node =
+      NodeLogger(
+          log: seq<LogEntry>
+      )
+    | NodeController(
+          leader: bool,
+          controllerState: ControllerState,
+          config: Config,
+
+          recved_events: map<SwitchIdPair, Event>,
+
+          log_copy: seq<LogEntry>
+      )
+    | NodeSwitch(
+          bufferedEvents: seq<Event>,
+          switchState: SwitchState,
+          event_id: int,
+          master: EndPoint
+      )
+
+  predicate NodeInit(node: Node, my_index: int, config: Config) {
+    (
+      node.NodeLogger? &&
+        node.log == []
+    ) || (
+      node.NodeController? &&
+        node.leader == (my_index == 0) &&
+        controllerStateInit(node.controllerState) &&
+        node.config == config
+    ) || (
+      node.NodeSwitch? &&
+        node.bufferedEvents == [] &&
+        switchStateInit(node.switchState) &&
+        node.event_id == 0 &&
+        |config.node_controllers| >= 1 &&
+        node.master == config.node_controllers[0]
+    )
+  }
+
+  predicate Node_SwitchEvent(s: Node, s': Node, event: Event, ios: seq<RavanaIo>) {
+    s.NodeSwitch? &&
+      s' == s.
+          (bufferedEvents := s.bufferedEvents + [event]).
+          (event_id := s.event_id + 1) &&
+      |ios| == 1 && ios[0].LIoOpSend? &&
+
+      var packet := ios[0].s;
+          packet.msg == EventMessage(event, s.event_id)
+       && packet.dst == s.master
+  }
+
+  predicate Node_ControllerLogEvent(s: Node, s': Node, ios: seq<RavanaIo>) {
+    s.NodeController? &&
+    s.leader &&
+    s' == s &&
+    |ios| == 2 &&
+    ios[0].LIoOpReceive? &&
+    ios[1].LIoOpSend? &&
+    var recv_packet := ios[0].r;
+    var send_packet := ios[1].s;
+
+    recv_packet.msg.EventMessage? &&
+
+    send_packet.dst == s.config.node_logger &&
+    send_packet.msg == LogMessage(LMRecv(
+        recv_packet.src, recv_packet.msg.event, recv_packet.msg.event_id))
+  }
+
+  // TODO get the log 
+
+  //predicate Node_ControllerProc
 }
