ironfleet/ravana/Types.i.dfy
@@ -1,5 +1,5 @@
-include "../../Common/Framework/Environment.s.dfy"
-include "../../Common/Native/Io.s.dfy"
+include "../src/Dafny/Distributed/Common/Framework/Environment.s.dfy"
+include "../src/Dafny/Distributed/Common/Native/Io.s.dfy"
 
 module Types_i {
   import opened Environment_s
@@ -8,7 +8,25 @@ module Types_i {
   type SwitchState
   type ControllerState
 
+  predicate controllerStateInit(cs: ControllerState)
+  predicate switchStateInit(ss: SwitchState)
+
+  type Event
+  type Command
+
   datatype RavanaMessage = 
+      EventMessage(event: Event, event_id: int)
+    | EventAck(event_ack_id: int)
+    | CommandMessage(command: Command, command_id: int)
+    | CommandAck(command_ack_id: int)
+    | NewMaster
+    | LogMessage(log_entry: LogEntry)
+
+  datatype LogEntry =
+      LMRecv(switch: EndPoint, event: Event, event_id: int)
+    | LMProc(comp_id: int)
+
+  datatype SwitchIdPair = SwitchIdPair(switch: EndPoint, event_id: int)
 
   type RavanaEnvironment = LEnvironment<EndPoint, RavanaMessage>
   type RavanaPacket = LPacket<EndPoint, RavanaMessage>
