ironfleet/ravana/compile.sh
@@ -1,0 +1,2 @@
+#!/bin/bash
+mono ../tools/Dafny/Dafny.exe Node.i.dfy
